tout casser

template-coq/theories/kernel/uGraph.v
@@ -6,19 +6,33 @@ From Template Require Import utils config Universes wGraph monad_utils.
 Import ConstraintType. Import MonadNotation.
 Local Open Scope nat_scope.
 
+Lemma iff_forall {A} B C (H : forall x : A, B x <-> C x)
+  : (forall x, B x) <-> (forall x, C x).
+  firstorder.
+Defined.
+
+Lemma iff_ex {A} B C (H : forall x : A, B x <-> C x)
+  : (ex B) <-> (ex C).
+  firstorder.
+Defined.
+
+Lemma if_true_false (b : bool) : (if b then true else false) = b.
+  destruct b; reflexivity.
+Qed.
+
 
 Module ConstraintSetFact := WFactsOn UnivConstraintDec ConstraintSet.
 Module ConstraintSetProp := WPropertiesOn UnivConstraintDec ConstraintSet.
 
 
 
-Inductive my_level := mLevel (_ : string) | mVar (_ : nat).
+Inductive gc_level := mLevel (_ : string) | mVar (_ : nat).
 
 Inductive good_constraint :=
 (* l <= l' *)
-| gc_le : my_level -> my_level -> good_constraint
+| gc_le : gc_level -> gc_level -> good_constraint
 (* l < l' *)
-| gc_lt : my_level -> my_level -> good_constraint
+| gc_lt : gc_level -> gc_level -> good_constraint
 (* Set < Var n *)
 | gc_lt_set : nat -> good_constraint
 (* Set = Var n *)
@@ -29,12 +43,12 @@ Module GoodConstraintDec.
   Definition t : Set := good_constraint.
   Definition eq : t -> t -> Prop := eq.
   Definition eq_equiv : RelationClasses.Equivalence eq := _.
-  Definition my_level_dec : forall x y : my_level, {x = y} + {x <> y}.
+  Definition gc_level_dec : forall x y : gc_level, {x = y} + {x <> y}.
     decide equality. apply string_dec. apply Peano_dec.eq_nat_dec.
   Defined.
   Definition eq_dec : forall x y : t, {eq x y} + {~ eq x y}.
     unfold eq.
-    decide equality. all: try apply my_level_dec.
+    decide equality. all: try apply gc_level_dec.
     all: apply Peano_dec.eq_nat_dec.
   Defined.
 End GoodConstraintDec.
@@ -44,6 +58,34 @@ Module GoodConstraintSetProp := WPropertiesOn GoodConstraintDec GoodConstraintSe
 
 Definition GoodConstraintSet_pair x y
   := GoodConstraintSet.add y (GoodConstraintSet.singleton x).
+
+Definition gc_val0 (v : valuation) (l : gc_level) : nat :=
+  match l with
+  | mLevel s => Pos.to_nat (v.(valuation_mono) s)
+  | mVar x => v.(valuation_poly) x
+  end.
+
+Definition gc_satisfies0 v (gc : good_constraint) : bool :=
+  match gc with
+  | gc_le l l' => gc_val0 v l <=? gc_val0 v l'
+  | gc_lt l l' => gc_val0 v l <? gc_val0 v l'
+  | gc_lt_set l => 0 <? v.(valuation_poly) l
+  | gc_eq_set l => 0 =? v.(valuation_poly) l
+  end.
+
+Definition gc_satisfies v : GoodConstraintSet.t -> bool :=
+  GoodConstraintSet.for_all (gc_satisfies0 v).
+
+Definition gc_consistent ctrs : Prop := exists v, gc_satisfies v ctrs.
+
+Lemma gc_satisfies_pair v gc1 gc2 :
+  (gc_satisfies0 v gc1 /\ gc_satisfies0 v gc2) <->
+  gc_satisfies v (GoodConstraintSet_pair gc1 gc2).
+Proof.
+  cbn; destruct (GoodConstraintDec.eq_dec gc2 gc1); cbn;
+    rewrite if_true_false.
+  now destruct e. symmetry. apply andb_and.
+Defined.
 
 (* None -> not satisfiable *)
 (* Some empty -> useless *)
@@ -75,15 +117,19 @@ Definition gc_of_constraint (uc : univ_constraint) : option GoodConstraintSet.t
      (* Level _ _ *)
      | (Level.Level _, Le, Level.lProp) => None
      | (Level.Level _, Le, Level.lSet) => None
-     | (Level.Level l, Le, Level.Level l') => singleton (gc_le (mLevel l) (mLevel l'))
+     | (Level.Level l, Le, Level.Level l')
+       => singleton (gc_le (mLevel l) (mLevel l'))
      | (Level.Level l, Le, Level.Var n) => singleton (gc_le (mLevel l) (mVar n))
      | (Level.Level _, Eq, Level.lProp) => None
      | (Level.Level _, Eq, Level.lSet) => None
-     | (Level.Level l, Eq, Level.Level l') => pair (gc_le (mLevel l) (mLevel l')) (gc_le (mLevel l') (mLevel l))
-     | (Level.Level l, Eq, Level.Var n) => pair (gc_le (mLevel l) (mVar n)) (gc_le (mVar n) (mLevel l))
+     | (Level.Level l, Eq, Level.Level l')
+       => pair (gc_le (mLevel l) (mLevel l')) (gc_le (mLevel l') (mLevel l))
+     | (Level.Level l, Eq, Level.Var n)
+       => pair (gc_le (mLevel l) (mVar n)) (gc_le (mVar n) (mLevel l))
      | (Level.Level _, Lt, Level.lProp) => None
      | (Level.Level _, Lt, Level.lSet) => None
-     | (Level.Level l, Lt, Level.Level l') => singleton (gc_lt (mLevel l) (mLevel l'))
+     | (Level.Level l, Lt, Level.Level l')
+       => singleton (gc_lt (mLevel l) (mLevel l'))
      | (Level.Level l, Lt, Level.Var n) => singleton (gc_lt (mLevel l) (mVar n))
 
      (* Var _ _ *)
@@ -93,46 +139,16 @@ Definition gc_of_constraint (uc : univ_constraint) : option GoodConstraintSet.t
      | (Level.Var n, Le, Level.Var n') => singleton (gc_le (mVar n) (mVar n'))
      | (Level.Var _, Eq, Level.lProp) => None
      | (Level.Var n, Eq, Level.lSet) => singleton (gc_eq_set n)
-     | (Level.Var n, Eq, Level.Level l) => pair (gc_le (mVar n) (mLevel l)) (gc_le (mLevel l) (mVar n))
+     | (Level.Var n, Eq, Level.Level l)
+       => pair (gc_le (mVar n) (mLevel l)) (gc_le (mLevel l) (mVar n))
 
-     | (Level.Var n, Eq, Level.Var n') => pair (gc_le (mVar n) (mVar n')) (gc_le (mVar n') (mVar n))
+     | (Level.Var n, Eq, Level.Var n')
+       => pair (gc_le (mVar n) (mVar n')) (gc_le (mVar n') (mVar n))
      | (Level.Var _, Lt, Level.lProp) => None
      | (Level.Var _, Lt, Level.lSet) => None
      | (Level.Var n, Lt, Level.Level l) => singleton (gc_lt (mVar n) (mLevel l))
      | (Level.Var n, Lt, Level.Var n') => singleton (gc_lt (mVar n) (mVar n'))
      end.
-
-Definition gc_val0 (v : valuation) (l : gc_level) : nat :=
-  match l with
-  | mLevel s => Pos.to_nat (v.(valuation_mono) s)
-  | mVar x => v.(valuation_poly) x
-  end.
-
-Definition gc_satisfies0 v (gc : good_constraint) : bool :=
-  match gc with
-  | gc_le l l' => gc_val0 v l <=? gc_val0 v l'
-  | gc_lt l l' => gc_val0 v l <? gc_val0 v l'
-  | gc_lt_set l => 0 <? v.(valuation_poly) l
-  | gc_eq_set l => 0 =? v.(valuation_poly) l
-  end.
-
-Definition gc_satisfies v : GoodConstraintSet.t -> bool :=
-  GoodConstraintSet.for_all (gc_satisfies0 v).
-
-Definition gc_consistent ctrs : Prop := exists v, gc_satisfies v ctrs.
-
-Lemma if_true_false (b : bool) : (if b then true else false) = b.
-  destruct b; reflexivity.
-Qed.
-
-Lemma gc_satisfies_pair v gc1 gc2 :
-  (gc_satisfies0 v gc1 /\ gc_satisfies0 v gc2) <->
-  gc_satisfies v (GoodConstraintSet_pair gc1 gc2).
-Proof.
-  cbn; destruct (GoodConstraintDec.eq_dec gc2 gc1); cbn;
-    rewrite if_true_false.
-  now destruct e. symmetry. apply andb_and.
-Defined.
 
 
 Ltac gc_of_constraint_tac :=
@@ -172,11 +188,6 @@ Definition gc_of_constraints (ctrs : constraints) : option GoodConstraintSet.t
   := ConstraintSet.fold add_gc_of_constraint
                         ctrs (Some GoodConstraintSet.empty).
 
-
-Lemma iff_forall {A} B C (H : forall x : A, B x <-> C x)
-  : (forall x, B x) <-> (forall x, C x).
-  firstorder.
-Defined.
 
 Lemma gc_of_constraints_spec v ctrs :
   satisfies v ctrs <-> on_Some (gc_satisfies v) (gc_of_constraints ctrs).
@@ -257,6 +268,7 @@ Module VerticeDec.
   Definition eqb : t -> t -> bool := fun x y => if eq_dec x y then true else false.
 End VerticeDec.
 
+
 Module Import wGraph := wGraph.WeightedGraph VerticeDec.
 
 Definition init_graph := (VSet.singleton lSet, EdgeSet.empty, lSet).
@@ -283,20 +295,151 @@ Definition EdgeSet_triple x y z
 
 Definition edges_of_constraint (gc : good_constraint) : list EdgeSet.elt :=
   match gc with
-  | gc_le l l' => [(edge_of_level l); (edge_of_level l'); (ltv l, 0, ltv l')]
-  | gc_lt l l' => [(edge_of_level l); (edge_of_level l'); (ltv l, 1, ltv l')]
+  | gc_le l l' => [edge_of_level l; edge_of_level l'; (ltv l, 0, ltv l')]
+  | gc_lt l l' => [edge_of_level l; edge_of_level l'; (ltv l, 1, ltv l')]
   | gc_lt_set n => [(lSet, 1, ltv (mVar n))]
   | gc_eq_set n => [(ltv (mVar n), 0, lSet); (lSet, 0, ltv (mVar n))]
   end.
 
 Definition add_edges edges := fold_left add_edge edges.
 
-Lemma add_edges_invariants {G} (HG : invariants G) {gc}
+Ltac sets_iff :=
+  match goal with
+  |  |- (_ /\ _) <-> _
+     => eapply and_iff_compat_l; sets_iff
+  |  |- (_ /\ _) <-> _
+     => eapply and_iff_compat_l; sets_iff
+  |  |- (_ \/ _) <-> _
+     => eapply or_iff_compat_l; sets_iff
+  |  |- (_ \/ _) <-> _
+     => eapply or_iff_compat_l; sets_iff
+  |  |- VSet.In _ (VSet.add _ _) <-> _
+     => etransitivity; [eapply VSet.add_spec|sets_iff]
+  |  |- EdgeSet.In _ (EdgeSet.add _ _) <-> _
+     => etransitivity; [eapply EdgeSet.add_spec|sets_iff]
+  |  |- VSet.In _ (VSet.singleton _) <-> _
+     => etransitivity; [eapply VSet.singleton_spec|sets_iff]
+  |  |- EdgeSet.In _ (EdgeSet.singleton _) <-> _
+     => etransitivity; [eapply EdgeSet.singleton_spec|sets_iff]
+  | _ => reflexivity
+  end.
+
+Ltac simplify_sets :=
+  repeat match goal with
+  | |- VSet.In ?A (VSet.add ?B ?C)
+    => let X := fresh in
+      simple refine (let X : VSet.In A (VSet.add B C) <-> _ := _ in _);
+      [|sets_iff|apply (proj2 X); clear X]
+  | |- EdgeSet.In ?A (EdgeSet.add ?B ?C)
+    => let X := fresh in
+      simple refine (let X : EdgeSet.In A (EdgeSet.add B C) <-> _ := _ in _);
+      [|sets_iff|apply (proj2 X); clear X]
+  | H : VSet.In ?A (VSet.add ?B ?C) |- _
+    => let X := fresh in
+      simple refine (let X : VSet.In A (VSet.add B C) <-> _ := _ in _);
+      [|sets_iff|apply (proj1 X) in H; clear X]
+  | H : EdgeSet.In ?A (EdgeSet.add ?B ?C) |- _
+    => let X := fresh in
+      simple refine (let X : EdgeSet.In A (EdgeSet.add B C) <-> _ := _ in _);
+      [|sets_iff|apply (proj1 X) in H; clear X]
+  | H : VSet.In ?A (VSet.singleton ?B) |- _
+    => let X := fresh in
+      simple refine (let X : VSet.In A (VSet.singleton B) <-> _ := _ in _);
+      [|sets_iff|apply (proj1 X) in H; clear X]
+  | H : EdgeSet.In ?A (EdgeSet.singleton ?B) |- _
+    => let X := fresh in
+      simple refine (let X : EdgeSet.In A (EdgeSet.singleton B) <-> _ := _ in _);
+      [|sets_iff|apply (proj1 X) in H; clear X]
+  | H : EdgeSet.In ?A EdgeSet.empty |- _
+    => apply EdgeSetFact.empty_iff in H; contradiction
+  end.
+
+  
+
+
+Lemma add_edges_invariants {G} (HG : invariants G) (HG' : wGraph.s G = lSet) {gc}
   : invariants (add_edges (edges_of_constraint gc) G).
 Proof.
   destruct HG as [H1 [H2 H3]].
-  repeat split.
-Admitted.
+  destruct gc.
+  - repeat split; cbn in *; rewrite HG' in *; clear HG'.
+    + simplify_sets.
+      destruct H. left; subst; reflexivity.
+      right; right; destruct H. left; subst; reflexivity.
+      right; right; destruct H. left; subst; reflexivity.
+      right; right. firstorder.
+    + simplify_sets.
+      right; destruct H. left; subst; reflexivity.
+      right; right; destruct H. left; subst; reflexivity.
+      right; right; destruct H. left; subst; reflexivity.
+      right. firstorder.
+    + simplify_sets. repeat right; assumption.
+    + intros x H; cbn; simplify_sets.
+      match goal with
+      | |- Rs ?X _ _ => set (G' := X)
+      end.
+      assert (R G' lSet g). {
+        destruct g; eexists; cbn; simplify_sets; eauto. }
+      assert (R G' lSet g0). {
+        destruct g0; eexists; cbn; simplify_sets; eauto. }
+      intuition; subst; try (constructor; assumption). 
+      1-2: destruct g0; try reflexivity; try (constructor; assumption).
+      1-2: destruct g; try reflexivity; try (constructor; assumption).
+      repeat apply Rs_add_edge; firstorder.
+  (* This bullet is a copy and paste of the first one *)
+  - repeat split; cbn in *; rewrite HG' in *; clear HG'.
+    + simplify_sets.
+      destruct H. left; subst; reflexivity.
+      right; right; destruct H. left; subst; reflexivity.
+      right; right; destruct H. left; subst; reflexivity.
+      right; right. firstorder.
+    + simplify_sets.
+      right; destruct H. left; subst; reflexivity.
+      right; right; destruct H. left; subst; reflexivity.
+      right; right; destruct H. left; subst; reflexivity.
+      right. firstorder.
+    + simplify_sets. repeat right; assumption.
+    + intros x H; cbn; simplify_sets.
+      match goal with
+      | |- Rs ?X _ _ => set (G' := X)
+      end.
+      assert (R G' lSet g). {
+        destruct g; eexists; cbn; simplify_sets; eauto. }
+      assert (R G' lSet g0). {
+        destruct g0; eexists; cbn; simplify_sets; eauto. }
+      intuition; subst; try (constructor; assumption). 
+      1-2: destruct g0; try reflexivity; try (constructor; assumption).
+      1-2: destruct g; try reflexivity; try (constructor; assumption).
+      repeat apply Rs_add_edge; firstorder.
+  - repeat split; cbn in *; rewrite HG' in *; clear HG'.
+    + simplify_sets.
+      destruct H. left; subst; reflexivity.
+      right; right. firstorder.
+    + simplify_sets.
+      right; destruct H. left; subst; reflexivity.
+      right. firstorder.
+    + simplify_sets. repeat right; assumption.
+    + intros x H; cbn; simplify_sets.
+      intuition; subst.
+      reflexivity.
+      constructor. exists 1. cbn; simplify_sets; auto.
+      apply Rs_add_edge; firstorder.
+  - repeat split; cbn in *; rewrite HG' in *; clear HG'.
+    + simplify_sets.
+      destruct H. left; subst; reflexivity.
+      right; right; destruct H. left; subst; reflexivity.
+      right; right. firstorder.
+    + simplify_sets.
+      right; destruct H. left; subst; reflexivity.
+      right; right; destruct H. left; subst; reflexivity.
+      right. firstorder.
+    + simplify_sets. left; reflexivity.
+    + intros x H; cbn; simplify_sets.
+      intuition; subst.
+      all: try reflexivity.
+      1-2: constructor; exists 0; cbn; simplify_sets; auto.
+      repeat apply Rs_add_edge; firstorder.
+Qed.
 
 
 Definition make_graph (ctrs : GoodConstraintSet.t) : t
@@ -314,51 +457,117 @@ Definition valuation_of_labelling (l : labelling) : valuation
   := {| valuation_mono := fun s => Pos.of_nat (l (ltv (mLevel s)));
         valuation_poly := fun n => l (ltv (mVar n)) |}.
 
+
+Lemma make_graph_ind (P : t -> Prop) (P0 : P init_graph)
+      (P1 : forall G gc, P G -> P (add_edges (edges_of_constraint gc) G))
+      : forall ctrs, P (make_graph ctrs).
+Proof.
+  unfold make_graph. intro ctrs. rewrite GoodConstraintSet.fold_spec.
+  set (G := init_graph) in *. clearbody G; revert G P0.
+  set (l := GoodConstraintSet.elements ctrs); induction l.
+  - easy.
+  - intros G P0; cbn. apply IHl. now apply P1.
+Qed.
+
+Definition add_edges_E := fold_left (fun E0 e => EdgeSet.add e E0).
+
+Lemma edges_add_edge G E :
+  wGraph.E (add_edges E G) = add_edges_E E (wGraph.E G).
+Proof.
+  revert G; induction E; cbn; intro G. reflexivity.
+  apply IHE.
+Qed.
+
+Lemma In_add_edges lE SE e
+  : EdgeSet.In e (add_edges_E lE SE) <-> In e lE \/ EdgeSet.In e SE.
+Proof.
+  revert SE. induction lE; cbn.
+  - intuition.
+  - intros SE; split; intro H.
+    pose proof (proj1 (IHlE _) H) as HH; clear IHlE H.
+    destruct HH. intuition. simplify_sets. destruct H; auto.
+    apply IHlE. destruct H as [[|]|].
+    right; simplify_sets. all: intuition.
+Qed.
+
+
+Lemma InA_In_eq {A} x (l : list A) : InA eq x l <-> In x l.
+Proof.
+  etransitivity. eapply InA_alt.
+  firstorder. now subst.
+Qed.
+
+
 Section Spec.
   Context (ctrs : GoodConstraintSet.t).
   Let G := make_graph ctrs.
 
-  Lemma make_graph_invariants : invariants G.
+  Lemma make_graph_invariants : invariants G /\ wGraph.s G = lSet.
   Proof.
-    subst G; unfold make_graph. rewrite GoodConstraintSet.fold_spec.
-    pose proof init_graph_invariants as HG.
-    set (G := init_graph) in *. clearbody G; revert G HG.
-    set (l := GoodConstraintSet.elements ctrs). induction l.
-    - easy.
-    - intros G HG; cbn. apply IHl. now apply add_edges_invariants.
+    subst G; apply make_graph_ind; clear ctrs.
+    - split. apply init_graph_invariants. reflexivity.
+    - intros G gc HG; split. 
+      + now apply add_edges_invariants.
+      + destruct HG as [_ HG]. clear -HG.
+        revert G HG.
+        induction (edges_of_constraint gc). easy.
+        intros G HG. cbn; apply IHl; assumption.
+  Qed.
+
+  Definition source_make_graph := proj2 make_graph_invariants.
+
+  Definition ltv_inj x y : ltv x = ltv y -> x = y.
+  Proof.
+    now inversion 1.
+  Defined.
+
+  Definition ltv_lSet x : ltv x <> lSet.
+  Proof.
+    now inversion 1.
+  Defined.
+
+  Lemma source_edge_of_level g : (edge_of_level g)..s = lSet.
+  Proof.
+    destruct g; reflexivity.
+  Qed.
+
+  Lemma target_edge_of_level g : (edge_of_level g)..t = g.
+  Proof.
+    destruct g; reflexivity.
   Qed.
 
   Definition make_graph_edge
     : forall x, VSet.In (ltv x) (wGraph.V G) -> EdgeSet.In (edge_of_level x) (wGraph.E G).
   Proof.
-    subst G; unfold make_graph. rewrite GoodConstraintSet.fold_spec.
-    set (G := init_graph) in *. 
-    assert (HG : forall x, VSet.In (ltv x) (wGraph.V G)
-                      -> EdgeSet.In (edge_of_level x) (wGraph.E G)). {
-      subst G. cbn. intros x H; apply VSet.singleton_spec in H.
-      inversion H. }
-    clearbody G; revert G HG.
-    set (l := GoodConstraintSet.elements ctrs). induction l.
-    - cbn. easy.
-    - intros G HG; cbn. apply IHl. intro x.
-      destruct a; cbn.
-      + destruct m, m0; cbn.
-  Admitted.
+    subst G; apply make_graph_ind; clear ctrs.
+    - cbn. intros x H. simplify_sets. inversion H.
+    - intros G gc HG l H.
+      destruct gc; cbn in *; simplify_sets.
+      + rewrite !source_edge_of_level, !target_edge_of_level in H. right.
+        destruct H. apply ltv_inj in H. subst; auto.
+        destruct H. apply ltv_inj in H. subst; auto.
+        destruct H. inversion H.
+        destruct H. apply ltv_inj in H. subst; auto.
+        destruct H. inversion H.
+        destruct H. apply ltv_inj in H. subst; auto.
+        firstorder.
+      + rewrite !source_edge_of_level, !target_edge_of_level in H. right.
+        destruct H. apply ltv_inj in H. subst; auto.
+        destruct H. apply ltv_inj in H. subst; auto.
+        destruct H. inversion H.
+        destruct H. apply ltv_inj in H. subst; auto.
+        destruct H. inversion H.
+        destruct H. apply ltv_inj in H. subst; auto.
+        firstorder.
+      + destruct H. inversion H.
+        destruct H. apply ltv_inj in H; subst. cbn. admit.
+        firstorder.
+      + destruct H. inversion H.
+        destruct H. apply ltv_inj in H; subst. auto.
+        destruct H. apply ltv_inj in H; subst. auto.
+        destruct H. inversion H. firstorder.
+  Abort.
 
-  Lemma source_make_graph : wGraph.s G = lSet.
-  Proof.
-    subst G; unfold make_graph. rewrite GoodConstraintSet.fold_spec.
-    set (G := init_graph). 
-    assert (HG : wGraph.s G = lSet) by reflexivity.
-    clearbody G; revert G HG.
-    induction (GoodConstraintSet.elements ctrs).
-    intros; assumption.
-    intros G HG; cbn. apply IHl.
-    clear -HG.
-    revert G HG. induction (edges_of_constraint a).
-    intros G HG; assumption.
-    intros G HG. cbn; apply IHl; assumption.
-  Qed.
 
   Lemma valuation_labelling_eq l (Hl : correct_labelling G l)
     : forall x, VSet.In x (wGraph.V G)
@@ -370,101 +579,133 @@ Section Spec.
       f_equal. apply source_make_graph.
     - destruct l0; cbn. 2: reflexivity.
       intro Hs. apply Nat2Pos.id.
-      apply make_graph_edge in Hs.
-      apply (proj2 Hl) in Hs; cbn in Hs. lia.
+      assert (HH: EdgeSet.In (lSet, 1, ltv (mLevel s)) (wGraph.E G)). {
+        clear l Hl; subst G. revert s Hs.
+        apply make_graph_ind; clear ctrs.
+        - intros l H; cbn in *; simplify_sets. inversion H.
+        - intros G gc HG l H.
+          destruct gc; cbn in *; simplify_sets.
+          + rewrite !source_edge_of_level, !target_edge_of_level in H. right.
+            destruct H. apply ltv_inj in H. subst; auto.
+            destruct H. apply ltv_inj in H. subst; auto.
+            destruct H. inversion H.
+            destruct H. apply ltv_inj in H. subst; auto.
+            destruct H. inversion H.
+            destruct H. apply ltv_inj in H. subst; auto.
+            firstorder.
+          + rewrite !source_edge_of_level, !target_edge_of_level in H. right.
+            destruct H. apply ltv_inj in H. subst; auto.
+            destruct H. apply ltv_inj in H. subst; auto.
+            destruct H. inversion H.
+            destruct H. apply ltv_inj in H. subst; auto.
+            destruct H. inversion H.
+            destruct H. apply ltv_inj in H. subst; auto.
+            firstorder.
+          + destruct H. inversion H.
+            destruct H. inversion H. firstorder.
+          + destruct H. inversion H.
+            destruct H. inversion H.
+            destruct H. inversion H.
+            destruct H. inversion H. firstorder. }
+      apply (proj2 Hl) in HH; cbn in HH. lia.
   Qed.
 
-  Lemma toto e :
-    EdgeSet.In e (wGraph.E G) <-> 
-    (exists l, e = edge_of_level l) \/ (GoodConstraintSet.Exists (fun gc => In e (edges_of_constraint gc)) ctrs).
-  Admitted.
 
-  Lemma make_graph_gc gc :
-    GoodConstraintSet.In gc ctrs
-    -> Forall (fun e => EdgeSet.In e (wGraph.E G)) (edges_of_constraint gc).
+  Lemma edges_make_graph :
+    wGraph.E G =
+    GoodConstraintSet.fold (fun gc E => add_edges_E (edges_of_constraint gc) E)
+                           ctrs EdgeSet.empty.
   Proof.
-    subst G; unfold make_graph. rewrite GoodConstraintSet.fold_spec.
-    intro H; apply GoodConstraintSetProp.FM.elements_1 in H.
-    set (l := GoodConstraintSet.elements ctrs) in *.
-    set (G := init_graph). 
-    assert (HG : In gc l
-        \/ Forall (fun e => EdgeSet.In e (wGraph.E G)) (edges_of_constraint gc)). {
-      left. apply InA_alt in H. now destruct H as [y [[]]]. }
-    clearbody G; revert G HG; clear H.
-    induction l.
-    - intros G []. inversion H. assumption.
-    - intros G HG; cbn. apply IHl.
-      destruct HG as [H1|H2].
-      + inversion_clear H1.
-        * right. subst.
-          destruct gc; cbn; repeat constructor.
-          admit.
-        * now left.
-      + right. admit.
+    subst G; unfold make_graph.
+    rewrite !GoodConstraintSet.fold_spec.
+    set (ctrs' := GoodConstraintSet.elements ctrs); clearbody ctrs'; clear ctrs.
+    set (G := init_graph).
+    change EdgeSet.empty with (wGraph.E G).
+    clearbody G; revert G.
+    induction ctrs'; cbn.
+    - reflexivity.
+    - intros G. rewrite IHctrs'. f_equal. apply edges_add_edge.
   Qed.
-    
-  Admitted.
 
-  (* TODO: This proof should be better written *)
+  Lemma edges_make_graph' e :
+    EdgeSet.In e (wGraph.E G) <-> 
+    (GoodConstraintSet.Exists (fun gc => In e (edges_of_constraint gc)) ctrs).
+  Proof.
+    rewrite edges_make_graph. clear G.
+    rewrite !GoodConstraintSet.fold_spec.
+    etransitivity. shelve.
+    eapply iff_ex.
+    intro x. eapply and_iff_compat_r. symmetry; etransitivity.
+    eapply GoodConstraintSetProp.FM.elements_iff. eapply InA_In_eq.
+    Unshelve.
+    set (ctrs' := GoodConstraintSet.elements ctrs) in *.
+    clearbody ctrs'; clear ctrs.
+    set (SE := EdgeSet.empty) in *.
+    transitivity ((exists gc, In gc ctrs' /\ In e (edges_of_constraint gc))
+                  \/ EdgeSet.In e SE).
+    2: etransitivity; [eapply or_iff_compat_l, EdgeSetFact.empty_iff|intuition].
+    clearbody SE; revert SE. induction ctrs'; cbn; intros SE; split.
+    - now right.
+    - firstorder.
+    - intro H. specialize (IHctrs' (add_edges_E (edges_of_constraint a) SE)).
+      apply proj1 in IHctrs'.
+      specialize (IHctrs' H); clear H.
+      destruct IHctrs'. left. firstorder.
+      apply In_add_edges in H. destruct H; firstorder.
+    - intro H. apply IHctrs'. clear -H.
+      eapply or_iff_compat_l. apply In_add_edges.
+      destruct H as [[gc [[H1|H1] H2]]|H]; subst; firstorder.
+  Qed.
+
+
   Lemma make_graph_spec v :
     gc_satisfies v ctrs <-> correct_labelling G (labelling_of_valuation v).
   Proof.
     unfold gc_satisfies, correct_labelling. split; intro H.
     - split. now rewrite source_make_graph.
-      intros e He. apply toto in He. induction He.
-      + destruct H0 as [[]]; cbn in H0; subst; cbn; lia.
-      + apply GoodConstraintSet.for_all_spec in H.
-        2: intros x y []; reflexivity.
-        destruct H0 as [[] [H1 H2]]; cbn in *.
-        * destruct H2 as [|[|[|[]]]].
-          -- destruct m; subst; cbn in *; lia.
-          -- destruct m0; subst; cbn in *; lia.
-          -- specialize (H _ H1); cbn in H. apply PeanoNat.Nat.leb_le in H.
-             subst; clear H1. destruct m, m0; simpl in *; lia.
-        * destruct H2 as [|[|[|[]]]].
-          -- destruct m; subst; cbn in *; lia.
-          -- destruct m0; subst; cbn in *; lia.
-          -- specialize (H _ H1); cbn in H.
-             case_eq (gc_val0 v m0). intro eq; rewrite eq in H.
-             discriminate.
-             intros n eq; rewrite eq in H.
-             apply PeanoNat.Nat.leb_le in H.
-             subst; clear H1. destruct m, m0; simpl in *; lia.
-        * destruct H2 as [|[]]. subst.
-          specialize (H _ H1); cbn in H.
-          case_eq (valuation_poly v n). intro eq; rewrite eq in H.
-          discriminate.
-          intros n0 eq; rewrite eq in H.
-          cbn. rewrite eq; lia.
-        * destruct H2 as [|[|[]]]. subst.
-          -- specialize (H _ H1); cbn in H.
-             case_eq (valuation_poly v n). intro eq; rewrite eq in H.
-             cbn. rewrite eq; lia.
-             intros n0 eq; rewrite eq in H; discriminate.
-          -- subst; cbn.
-             specialize (H _ H1); cbn in H.
-             case_eq (valuation_poly v n). intro; lia.
-             intros n0 eq; rewrite eq in H; discriminate.
+      intros e He. 
+      apply edges_make_graph' in He.
+      destruct He as [gc [H0 H1]].
+      apply GoodConstraintSet.for_all_spec in H.
+      2: intros x y []; reflexivity.
+      specialize (H _ H0). cbn in *.
+      clear -H H1.
+      destruct gc; try apply PeanoNat.Nat.leb_le in H.
+      + destruct H1; subst. rewrite source_edge_of_level.
+        destruct g; cbn; lia.
+        destruct H0; subst. rewrite source_edge_of_level.
+        destruct g0; cbn; lia.
+        destruct H0 as [|[]]; subst. destruct g, g0; cbn in *; lia.
+      + destruct H1; subst. rewrite source_edge_of_level.
+        destruct g; cbn; lia.
+        destruct H0; subst. rewrite source_edge_of_level.
+        destruct g0; cbn; lia.
+        destruct H0 as [|[]]; subst. destruct g, g0; cbn in *; lia.
+      + destruct H1 as [|[]]; subst. cbn. assumption. 
+      + destruct H1 as [|[|[]]]; subst; cbn.
+        apply PeanoNat.Nat.eqb_eq in H. lia. lia.
     - apply GoodConstraintSet.for_all_spec.
       intros x y []; reflexivity.
-      intros gc Hgc. apply tata in Hgc.
-      apply proj2 in H.
-      destruct gc; cbn in *.
-      + inversion_clear Hgc. inversion_clear H1. inversion_clear H3.
-        specialize (H _ H1); clear -H. cbn in *.
-        destruct m, m0; cbn; apply PeanoNat.Nat.leb_le; lia.
-      + inversion_clear Hgc. inversion_clear H1. inversion_clear H3.
-        specialize (H _ H1); clear -H. cbn in *.
-        case_eq (gc_val0 v m0); intro e.
-        destruct m, m0; cbn in *; lia.
-        intro ee. apply PeanoNat.Nat.leb_le.
-        destruct m, m0; cbn in *; lia.
-      + inversion_clear Hgc. specialize (H _ H0); clear -H. cbn in *.
-        case_eq (valuation_poly v n); intros; try reflexivity; lia.
-      + inversion_clear Hgc. specialize (H _ H0); clear -H. cbn in *.
-        case_eq (valuation_poly v n); intros; try reflexivity; lia.
+      intros gc Hgc.
+      pose proof (fun e p => proj2 (edges_make_graph' e)
+                                (ex_intro _ gc (conj Hgc p))) as H0.
+      destruct H as [_ H].
+      pose proof (fun e p => H e (H0 e p)) as HH. clear -HH.
+      destruct gc; cbn in HH; try apply PeanoNat.Nat.leb_le.
+      4: apply PeanoNat.Nat.eqb_eq.
+      simple refine (let HH' := HH (ltv g, 0, ltv g0) _ in _);
+        [intuition|clearbody HH'; clear HH];
+        destruct g, g0; cbn in *; lia.
+      simple refine (let HH' := HH (ltv g, 1, ltv g0) _ in _);
+        [intuition|clearbody HH'; clear HH];
+        destruct g, g0; cbn in *; lia.
+      simple refine (let HH' := HH (lSet, 1, ltv (mVar n)) _ in _);
+        [intuition|clearbody HH'; clear HH];
+        cbn in *; lia.
+      simple refine (let HH' := HH (ltv (mVar n), 0, lSet) _ in _);
+        [intuition|clearbody HH'; clear HH];
+        cbn in *; lia.
   Qed.
-
 
 
   Corollary make_graph_spec' l :
@@ -490,293 +731,61 @@ Section Spec.
 End Spec.
 
 
-
-
-
-
-
-
-
-
-
-
-
-
-
-
-
-
-
-  Definition check_le_vertice (l1 l2 : vertice) : bool :=
-    match enforce l1 l2 with
-    | Some k => Z.geb k 0
-    | None => false
-    end.
-
-  Definition check_lt_vertice (l1 l2 : vertice) : bool :=
-    match enforce l1 l2 with
-    | Some k => Z.geb k 1
-    | None => false
-    end.
-
-  Definition check_eq_vertice (l1 l2 : vertice) : bool :=
-    check_le_vertice l1 l2 && check_le_vertice l2 l1.
-
-
-  Definition check_le_level (l1 l2 : universe_level) : bool :=
-    match ltv l1, ltv l2 with
-    | None, _ => true
-    | _, None => false
-    | Some l1, Some l2 => match enforce l1 l2 with
-                         | Some k => Z.geb k 0
-                         | None => false
-                         end
-    end.
-
-  Definition check_lt_level (l1 l2 : universe_level) : bool :=
-    match ltv l1, ltv l2 with
-    | _, None => false
-    | None, _ => true
-    | Some l1, Some l2 => match enforce l1 l2 with
-                         | Some k => Z.geb k 1
-                         | None => false
-                         end
-    end.
-
-  Definition check_eq_level (l1 l2 : universe_level) : bool :=
-    check_le_level l1 l2 && check_le_level l2 l1.
-
-
-  Definition check_constraint (cstr : univ_constraint) : bool :=
-    let '(l, d, r) := cstr in
-    match d with
-    | Eq => check_eq_level l r
-    | Lt => check_lt_level l r
-    | Le => check_le_level l r
-    end.
-
-  Definition check_constraints (cstrs : ConstraintSet.t) : bool :=
-    ConstraintSet.for_all check_constraint cstrs.
-
-  Definition check_le_level_expr (e1 e2 : Universe.Expr.t) : bool :=
-    match ltv (fst e1), ltv (fst e2) with
-    | None, _ => true
-    | _, None => false
-    | Some l1, Some l2 =>
-      match enforce l1 l2 with
-      | None => false
-      | Some k => match snd e1, snd e2 with
-                 | false, false
-                 | true, true => k >=? 0
-                 | true, false => k >=? 1
-                 | false, true => k >=? -1
-                 end
-      end
-    end.
-
-  Definition check_lt_level_expr (e1 e2 : Universe.Expr.t) : bool :=
-    match ltv (fst e1), ltv (fst e2) with
-    | _, None => false
-    | None, _ => true
-    | Some l1, Some l2 =>
-      match enforce l1 l2 with
-      | None => false
-      | Some k => match snd e1, snd e2 with
-                 | false, false
-                 | true, true => k >=? 1
-                 | true, false => k >=? 2
-                 | false, true => k >=? 0
-                 end
-      end
-    end.
-
-  Definition check_eq_level_expr (e1 e2 : Universe.Expr.t) : bool :=
-    check_le_level_expr e1 e2 && check_le_level_expr e2 e1.
-
-  Definition exists_bigger_or_eq (e1 : Universe.Expr.t) (u2 : Universe.t) : bool :=
-    Universe.existsb (check_le_level_expr e1) u2.
-
-  Definition exists_strictly_bigger (e1 : Universe.Expr.t) (u2 : Universe.t) : bool :=
-    Universe.existsb (check_lt_level_expr e1) u2.
-
-  Definition check_lt (u1 u2 : Universe.t) : bool :=
-    Universe.for_all (fun e => exists_strictly_bigger e u2) u1.
-
-  Definition check_leq0 (u1 u2 : Universe.t) : bool :=
-    Universe.for_all (fun e => exists_bigger_or_eq e u2) u1.
-
-  (** We try syntactic equality before checking the graph. *)
-  Definition check_leq `{checker_flags} s s' :=
-    negb check_univs || Universe.equal s s' || check_leq0 s s'.
-
-  Definition check_eq `{checker_flags} s s' :=
-    negb check_univs || Universe.equal s s' || (check_leq0 s s' && check_leq0 s' s).
-
-  Definition check_eq_instance `{checker_flags} u v :=
-    Instance.equal_upto check_eq_level u v.
-
-End BellmanFord.
-
-
-Section Specif.
-  Conjecture no_universe_inconsistency_ok : forall φ, reflect (well_founded (R φ)) (no_universe_inconsistency φ).
-
-  Local Existing Instance default_checker_flags.
-
-  (* TODO: lower level conjecture *)
-  Conjecture check_leq_specif
-    : forall ctrs φ (e : make_graph ctrs = Some φ) u1 u2, reflect (leq_universe ctrs u1 u2) (check_leq φ u1 u2).
-
-  Conjecture check_eq_specif
-    : forall ctrs φ (e : make_graph ctrs = Some φ) u1 u2, reflect (eq_universe ctrs u1 u2) (check_eq φ u1 u2).
-End Specif.
-
-  (* Definition check_eq_refl `{checker_flags} u : check_eq φ u u = true. *)
-  (*   unfold check_eq; destruct check_univs; cbn; [|reflexivity]. *)
-
-  (* Conjecture eq_universe_instance_refl : forall `{checker_flags} u, eq_universe_instance u u = true. *)
-  (* Conjecture eq_universe_leq_universe : forall `{checker_flags} x y, *)
-  (*     eq_universe x y = true -> leq_universe x y = true. *)
-  (* Conjecture leq_universe_product_l : forall `{checker_flags} s1 s2, *)
-  (*     leq_universe s1 (Universe.sort_of_product s1 s2) = true. *)
-  (* Conjecture leq_universe_product_r : forall `{checker_flags} s1 s2, *)
-  (*     leq_universe s2 (Universe.sort_of_product s1 s2) = true. *)
-
-
-
-
-    (* Inductive super_result := *)
-    (* | SuperSame (_ : bool) *)
-    (* (* The level expressions are in cumulativity relation. boolean *)
-    (*        indicates if left is smaller than right?  *) *)
-    (* | SuperDiff (_ : comparison). *)
-    (* (* The level expressions are unrelated, the comparison result *)
-    (*        is canonical *) *)
-
-    (* (** [super u v] compares two level expressions, *)
-    (*    returning [SuperSame] if they refer to the same level at potentially different *)
-    (*    increments or [SuperDiff] if they are different. The booleans indicate if the *)
-    (*    left expression is "smaller" than the right one in both cases. *) *)
-    (* Definition super (x y : t) : super_result := *)
-    (*   match Level.compare (fst x) (fst y) with *)
-    (*   | Eq => SuperSame (bool_lt' (snd x) (snd y)) *)
-    (*   | cmp => *)
-    (*       match x, y with *)
-    (*       | (l, false), (l', false) => *)
-    (*         match l, l' with *)
-    (*         | Level.lProp, Level.lProp => SuperSame false *)
-    (*         | Level.lProp, _ => SuperSame true *)
-    (*         | _, Level.lProp => SuperSame false *)
-    (*         | _, _ => SuperDiff cmp *)
-    (*         end *)
-    (*       | _, _ => SuperDiff cmp *)
-    (*       end *)
-    (*   end. *)
-
-
-  (* Fixpoint merge_univs (fuel : nat) (l1 l2 : list Expr.t) : list Expr.t := *)
-  (*   match fuel with *)
-  (*   | O => l1 *)
-  (*   | S fuel => match l1, l2 with *)
-  (*              | [], _ => l2 *)
-  (*              | _, [] => l1 *)
-  (*              | h1 :: t1, h2 :: t2 => *)
-  (*                match Expr.super h1 h2 with *)
-  (*                | Expr.SuperSame true (* h1 < h2 *) => merge_univs fuel t1 l2 *)
-  (*                | Expr.SuperSame false => merge_univs fuel l1 t2 *)
-  (*                | Expr.SuperDiff Lt (* h1 < h2 is name order *) *)
-  (*                  => h1 :: (merge_univs fuel t1 l2) *)
-  (*                | _ => h2 :: (merge_univs fuel l1 t2) *)
-  (*                end *)
-  (*              end *)
-  (*   end. *)
-
-
-
-(* (* The monomorphic levels are > Set while polymorphic ones are >= Set. *) *)
-(* Definition add_node (l : Level.t) (G : t) : t *)
-(*   := let levels := LevelSet.add l (fst G) in *)
-(*      let constraints := *)
-(*          match l with *)
-(*          | Level.lProp | Level.lSet => snd G (* supposed to be yet here *) *)
-(*          | Level.Var _ => ConstraintSet.add (Level.set, ConstraintType.Le, l) (snd G) *)
-(*          | Level.Level _ => ConstraintSet.add (Level.set, ConstraintType.Lt, l) (snd G) *)
-(*          end in *)
-(*      (levels, constraints). *)
-
-(* Definition add_constraint (uc : univ_constraint) (G : t) : t *)
-(*   := let '((l, ct),l') := uc in *)
-(*      (* maybe useless if we always add constraints *)
-(*         in which the universes are declared *) *)
-(*      let G := add_node l (add_node l' G) in *)
-(*      let constraints := ConstraintSet.add uc (snd G) in *)
-(*      (fst G, constraints). *)
-
-(* Definition repr (uctx : universe_context) : UContext.t := *)
-(*   match uctx with *)
-(*   | Monomorphic_ctx c => c *)
-(*   | Polymorphic_ctx c => c *)
-(*   | Cumulative_ctx c => CumulativityInfo.univ_context c *)
-(*   end. *)
-
-(* Definition add_global_constraints (uctx : universe_context) (G : t) : t *)
-(*   := match uctx with *)
-(*      | Monomorphic_ctx (inst, cstrs) => *)
-(*        let G := List.fold_left (fun s l => add_node l s) inst G in *)
-(*        ConstraintSet.fold add_constraint cstrs G *)
-(*      | Polymorphic_ctx _ => G *)
-(*      | Cumulative_ctx _ => G *)
-(*      end. *)
-
-
-
-Section Test.
-
-  Definition get_graph G0 := match G0 with
-                             | Some φ => φ
-                             | None => init_graph
-                             end.
-
-  Definition G0 := make_graph ConstraintSet.empty.
-  Check (eq_refl : G0 = Some _).
-  Definition G := get_graph G0.
-
-  Local Existing Instance default_checker_flags.
-
-  Check (eq_refl : check_leq G Universe.type0m Universe.type0 = true).
-  Check (eq_refl : check_lt G Universe.type0m Universe.type0 = true).
-  Check (eq_refl : check_lt G Universe.type0m Universe.type0m = false).
-  Check (eq_refl : check_lt G Universe.type0 Universe.type0m = false).
-  Check (eq_refl : check_lt G Universe.type0 Universe.type0 = false).
-  Check (eq_refl : no_universe_inconsistency G = true).
-
-  Definition ctrs0 := ConstraintSet.add (Level.Level "Top.0", Lt, Level.Level "Top.1")
-                                        (ConstraintSet.singleton (Level.Var 0, Lt, Level.Var 1)).
-  Definition G'0 := make_graph ctrs0.
-  Check (eq_refl : G'0 = Some _).
-  Definition G' := get_graph G'0.
-
-  Check (eq_refl : check_lt G' (Universe.make (Level.Level "Top.0")) (Universe.make (Level.Var 0)) = false).
-  Check (eq_refl : check_leq G' (Universe.make (Level.Level "Top.1")) (Universe.make (Level.lProp)) = false).
-  Check (eq_refl : check_leq G' (Universe.super (Level.Level "Top.1")) (Universe.make (Level.Level "Top.1")) = false).
-  Check (eq_refl : check_lt G' (Universe.make (Level.Level "Top.1")) (Universe.super (Level.Level "Top.1")) = true).
-  Check (eq_refl : check_lt G' (Universe.make (Level.Level "Top.1")) (Universe.make (Level.Level "Top.1")) = false).
-  Check (eq_refl : check_eq G' (Universe.make (Level.Level "Top.1")) (Universe.make (Level.Level "Top.1")) = true).
-  Check (eq_refl : no_universe_inconsistency G = true).
-
-  Check (eq_refl : check_lt G' (Universe.make (Level.Var 1)) (Universe.make (Level.Var 0)) = false).
-  Check (eq_refl : check_leq G' (Universe.make (Level.Var 0)) (Universe.make (Level.Var 1)) = true).
-  Check (eq_refl : check_lt G' (Universe.make (Level.Var 0)) (Universe.make (Level.Var 1)) = true).
-  Check (eq_refl : check_leq G' Universe.type1 Universe.type0 = false).
-  Check (eq_refl : check_lt G' Universe.type1 Universe.type1 = false).
-
-
-  Definition ctrs1 := ConstraintSet.add (Level.Var 1, Eq, Level.Var 2)
-                                        (ConstraintSet.add (Level.Var 2, Le, Level.lSet) ctrs0).
-  Definition G''0 := make_graph ctrs1.
-  Check (eq_refl : G''0 = Some _).
-  Definition G'' := get_graph G''0.
-
-  Check (eq_refl : no_universe_inconsistency G'' = false).
-
-End Test.
+Definition G := make_graph
+  (GoodConstraintSet.add (gc_lt (mVar 0) (mVar 1))
+ (GoodConstraintSet_pair (gc_lt_set 0) (gc_lt_set 1))).
+
+Compute (d' G lSet (mVar 0)).
+Compute (d' G lSet (mVar 1)).
+Compute (d' G lSet lSet).
+
+(* Section Test. *)
+
+(*   Definition get_graph G0 := match G0 with *)
+(*                              | Some φ => φ *)
+(*                              | None => init_graph *)
+(*                              end. *)
+
+(*   Definition G0 := make_graph ConstraintSet.empty. *)
+(*   Check (eq_refl : G0 = Some _). *)
+(*   Definition G := get_graph G0. *)
+
+(*   Local Existing Instance default_checker_flags. *)
+
+(*   Check (eq_refl : check_leq G Universe.type0m Universe.type0 = true). *)
+(*   Check (eq_refl : check_lt G Universe.type0m Universe.type0 = true). *)
+(*   Check (eq_refl : check_lt G Universe.type0m Universe.type0m = false). *)
+(*   Check (eq_refl : check_lt G Universe.type0 Universe.type0m = false). *)
+(*   Check (eq_refl : check_lt G Universe.type0 Universe.type0 = false). *)
+(*   Check (eq_refl : no_universe_inconsistency G = true). *)
+
+(*   Definition ctrs0 := ConstraintSet.add (Level.Level "Top.0", Lt, Level.Level "Top.1") *)
+(*                                         (ConstraintSet.singleton (Level.Var 0, Lt, Level.Var 1)). *)
+(*   Definition G'0 := make_graph ctrs0. *)
+(*   Check (eq_refl : G'0 = Some _). *)
+(*   Definition G' := get_graph G'0. *)
+
+(*   Check (eq_refl : check_lt G' (Universe.make (Level.Level "Top.0")) (Universe.make (Level.Var 0)) = false). *)
+(*   Check (eq_refl : check_leq G' (Universe.make (Level.Level "Top.1")) (Universe.make (Level.lProp)) = false). *)
+(*   Check (eq_refl : check_leq G' (Universe.super (Level.Level "Top.1")) (Universe.make (Level.Level "Top.1")) = false). *)
+(*   Check (eq_refl : check_lt G' (Universe.make (Level.Level "Top.1")) (Universe.super (Level.Level "Top.1")) = true). *)
+(*   Check (eq_refl : check_lt G' (Universe.make (Level.Level "Top.1")) (Universe.make (Level.Level "Top.1")) = false). *)
+(*   Check (eq_refl : check_eq G' (Universe.make (Level.Level "Top.1")) (Universe.make (Level.Level "Top.1")) = true). *)
+(*   Check (eq_refl : no_universe_inconsistency G = true). *)
+
+(*   Check (eq_refl : check_lt G' (Universe.make (Level.Var 1)) (Universe.make (Level.Var 0)) = false). *)
+(*   Check (eq_refl : check_leq G' (Universe.make (Level.Var 0)) (Universe.make (Level.Var 1)) = true). *)
+(*   Check (eq_refl : check_lt G' (Universe.make (Level.Var 0)) (Universe.make (Level.Var 1)) = true). *)
+(*   Check (eq_refl : check_leq G' Universe.type1 Universe.type0 = false). *)
+(*   Check (eq_refl : check_lt G' Universe.type1 Universe.type1 = false). *)
+
+
+(*   Definition ctrs1 := ConstraintSet.add (Level.Var 1, Eq, Level.Var 2) *)
+(*                                         (ConstraintSet.add (Level.Var 2, Le, Level.lSet) ctrs0). *)
+(*   Definition G''0 := make_graph ctrs1. *)
+(*   Check (eq_refl : G''0 = Some _). *)
+(*   Definition G'' := get_graph G''0. *)
+
+(*   Check (eq_refl : no_universe_inconsistency G'' = false). *)
+
+(* End Test. *)
